Monads shall define their weak equality relation

theories/Control.v
@@ -4,6 +4,8 @@ Require Import Coq.Classes.Equivalence.
 
 Require Import FreeSpec.WEq.
 
+Local Open Scope free_weq_scope.
+
 Polymorphic Definition compose
             {a b c: Type}
             (g: b -> c)
@@ -21,29 +23,85 @@ Polymorphic Definition id
 Notation "f <<< g" := (compose g f) (at level 50).
 Notation "f >>> g" := (compose f g) (at level 50).
 
+Definition function_weq
+           {a b: Type}
+          `{WEq b}
+           (f g: a -> b)
+  : Prop :=
+  forall (x: a), f x == g x.
+
+Lemma function_weq_refl
+      {a b: Type}
+     `{WEq b}
+      (f: a -> b)
+  : function_weq f f.
+Proof.
+  intro x.
+  reflexivity.
+Qed.
+
+Lemma function_weq_sym
+      {a b: Type}
+     `{WEq b}
+      (f g: a -> b)
+  : function_weq f g
+    -> function_weq g f.
+Proof.
+  unfold function_weq.
+  intros H' x.
+  rewrite H'.
+  reflexivity.
+Qed.
+
+Lemma function_weq_trans
+      {a b: Type}
+     `{WEq b}
+      (f g h: a -> b)
+  : function_weq f g
+    -> function_weq g h
+    -> function_weq f h.
+Proof.
+  unfold function_weq.
+  intros F G x.
+  rewrite <- (G x).
+  exact (F x).
+Qed.
+
+Add Parametric Relation
+    (a b: Type)
+   `{WEq b}
+  : (a -> b) (function_weq)
+    reflexivity  proved by function_weq_refl
+    symmetry     proved by function_weq_sym
+    transitivity proved by function_weq_trans
+      as function_web_equiv.
+
 Instance function_WEq
          (a b: Type)
+        `{WEq b}
   : WEq (a -> b) :=
-  { weq := eq
+  { weq := function_weq
   }.
 
 (** * Functor
 
  *)
 
-Local Open Scope free_weq_scope.
-
 Class Functor
       (f: Type -> Type)
-  := { functor_has_eq :> forall {a}, WEq (f a)
+  := { functor_has_eq :> forall {a: Type}
+                               `{WEq a},
+           WEq (f a)
      ; map {a b: Type}
            (g:   a -> b)
            (x:   f a)
        : f b
      ; functor_identity {a: Type}
+                       `{WEq a}
                         (x: f a)
        : map (@id a) x == id x
      ; functor_composition_identity {a b c: Type}
+                                   `{WEq c}
                                     (u:     a -> b)
                                     (v:     b -> c)
                                     (x:     f a)
@@ -51,8 +109,8 @@ Class Functor
      }.
 
 Arguments map [f _ a b] (_ _).
-Arguments functor_identity [f _ a].
-Arguments functor_composition_identity [f _ a].
+Arguments functor_identity [f _ a _] (x).
+Arguments functor_composition_identity [f _ a b c _] (u v x).
 
 Notation "f <$> g" :=
   (map f g)
@@ -73,14 +131,15 @@ Class Apply
          -> f b
        where "f <*> g" := (apply f g)
      ; apply_associative_composition: forall {a b c: Type}
+                                            `{WEq c}
                                              (u: f (b -> c))
                                              (v: f (a -> b))
                                              (w:   f a),
          compose <$> u <*> v <*> w == u <*> (v <*> w)
      }.
 
-Arguments apply [f _ a b].
-Arguments apply_associative_composition [f _ a b c] (u v w).
+Arguments apply [f _ a b] (_ _).
+Arguments apply_associative_composition [f _ a b c _] (u v w).
 
 Notation "f <*> g" :=
   (apply f g)
@@ -96,28 +155,32 @@ Class Applicative
      ; pure: forall {a: Type},
          a -> f a
      ; applicative_identity: forall {a: Type}
+                                   `{WEq a}
                                     (v: f a),
          pure id <*> v == v
      ; applicative_composition: forall {a b c: Type}
+                                      `{WEq c}
                                        (u:     f (b -> c))
                                        (v:     f (a -> b))
                                        (w:     f a),
          pure compose <*> u <*> v <*> w == u <*> (v <*> w)
      ; applicative_homomorphism: forall {a b: Type}
+                                       `{WEq b}
                                         (v:   a -> b)
                                         (x:   a),
          (pure v) <*> (pure x) == pure (v x)
      ; applicative_interchange: forall {a b: Type}
+                                      `{WEq b}
                                        (u: f (a -> b))
                                        (y: a),
          u <*> (pure y) == (pure (fun z => z y)) <*> u
      }.
 
 Arguments pure [f _ a] (x).
-Arguments applicative_identity [f _ a] (v).
-Arguments applicative_composition [f _ a b c] (u v w).
-Arguments applicative_homomorphism [f _ a b] (v x).
-Arguments applicative_interchange [f _ a b] (u y).
+Arguments applicative_identity [f _ a _] (v).
+Arguments applicative_composition [f _ a b c _] (u v w).
+Arguments applicative_homomorphism [f _ a b _] (v x).
+Arguments applicative_interchange [f _ a b _] (u y).
 
 (** * Bind
 
@@ -134,15 +197,15 @@ Class Bind
          -> m b
        where "f >>= g" := (bind f g)
      ; bind_associativity: forall {a b c: Type}
+                                 `{WEq c}
                                   (f:     m a)
                                   (g:     a -> m b)
                                   (h:     b -> m c),
          (f >>= g) >>= h == f >>= (fun x => (g x) >>= h)
-
      }.
 
 Arguments bind [m _ a b] (f g).
-Arguments bind_associativity [m _ a b c] (f g h).
+Arguments bind_associativity [m _ a b c _] (f g h).
 
 Notation "f >>= g" := (bind f g) (at level 28, left associativity).
 
@@ -163,16 +226,18 @@ Class Monad
   := { monad_is_applicative :> Applicative m
      ; monad_is_bind :> Bind m
      ; monad_left_identity: forall {a b: Type}
+                                  `{WEq b}
                                    (x:   a)
                                    (f:   a -> m b),
          pure x >>= f == f x
      ; monad_right_identity: forall {a: Type}
+                                   `{WEq a}
                                     (x: m a),
          x >>= (fun y => pure y) == x
      }.
 
-Arguments monad_left_identity [m _ a b] (x f).
-Arguments monad_right_identity [m _ a] (x).
+Arguments monad_left_identity [m _ a b _] (x f).
+Arguments monad_right_identity [m _ a _] (x).
 
 (** * Monad Transformer
 
