theories/Control/Identity.v
@@ -1,15 +1,113 @@
 Require Import FreeSpec.Control.
 Require Import FreeSpec.WEq.
 
-Definition Identity
-           (a: Type)
-  := a.
+Local Open Scope free_weq_scope.
+
+Inductive Identity
+          (a: Type)
+  : Type :=
+| identity (x: a)
+  : Identity a.
+
+Arguments identity [a] (x).
+
+Definition unwrap
+           {a: Type}
+           (x: Identity a)
+  : a :=
+  match x with
+  | identity x => x
+  end.
+
+Notation "! a" :=
+  (unwrap a)
+    (at level 41, right associativity).
+
+Definition identity_weq
+           {a: Type}
+          `{WEq a}
+           (x y: Identity a)
+  : Prop :=
+  !x == !y.
+
+Lemma identity_weq_refl
+      {a: Type}
+     `{WEq a}
+      (x: Identity a)
+  : identity_weq x x.
+Proof.
+  unfold identity_weq.
+  reflexivity.
+Qed.
+
+Lemma identity_weq_sym
+      {a: Type}
+     `{WEq a}
+      (x y: Identity a)
+  : identity_weq x y
+    -> identity_weq y x.
+Proof.
+  unfold identity_weq.
+  intro H'.
+  symmetry.
+  exact H'.
+Qed.
+
+Lemma identity_weq_trans
+      {a: Type}
+     `{WEq a}
+      (x y z: Identity a)
+  : identity_weq x y
+    -> identity_weq y z
+    -> identity_weq x z.
+Proof.
+  unfold identity_weq.
+  intros X Y.
+  rewrite X.
+  exact Y.
+Qed.
+
+Add Parametric Relation
+    (a: Type)
+   `{WEq a}
+  : (Identity a) (identity_weq)
+    reflexivity  proved by identity_weq_refl
+    symmetry     proved by identity_weq_sym
+    transitivity proved by identity_weq_trans
+      as identity_weq_equiv.
 
 Instance identity_WEq
          (a: Type)
+        `{WEq a}
   : WEq (Identity a) :=
-  { weq := eq
+  { weq := identity_weq
   }.
+
+Lemma wrap_unwrap_identity
+      {a: Type}
+     `{WEq a}
+      (x: Identity a)
+  : identity (! x) == x.
+Proof.
+  destruct x.
+  reflexivity.
+Qed.
+
+Lemma wrap_identity_weq
+      {a: Type}
+     `{WEq a}
+     (x y: a)
+  : x == y <-> identity x == identity y.
+Proof.
+  split.
+  + intro Heq.
+    cbn; unfold identity_weq.
+    exact Heq.
+  + intro Heq.
+    cbn in *.
+    unfold identity_weq in Heq.
+    exact Heq.
+Qed.
 
 (** * Functor
 
@@ -20,15 +118,19 @@ Definition identity_map
            (f:   a -> b)
            (x:   Identity a)
   : Identity b :=
-  f x.
+  identity (f (!x)).
 
 Instance identity_Functor
   : Functor Identity :=
   { map := identity_map
   }.
 Proof.
-  + reflexivity.
-  + reflexivity.
+  + intros a H x.
+    unfold identity_map; unfold id.
+    apply wrap_unwrap_identity.
+  + intros a b c H u v x.
+    apply wrap_identity_weq.
+    reflexivity.
 Defined.
 
 Definition identity_apply
@@ -36,31 +138,33 @@ Definition identity_apply
            (f:   Identity (a -> b))
            (x:   Identity a)
   : Identity b :=
-  f x.
+  identity ((!f) (!x)).
 
 Instance identity_Apply
   : Apply Identity :=
   { apply := identity_apply
   }.
 Proof.
-  + reflexivity.
+  + intros a b c HWEq u v w.
+    apply wrap_identity_weq.
+    reflexivity.
 Defined.
 
 Definition identity_pure
            (a: Type)
            (x: a)
   : Identity a :=
-  x.
+  identity x.
 
 Instance identity_Applicative
   : Applicative Identity :=
   { pure := identity_pure
   }.
 Proof.
-  + reflexivity.
-  + reflexivity.
-  + reflexivity.
-  + reflexivity.
+  + intros; apply <- wrap_identity_weq; reflexivity.
+  + intros; apply <- wrap_identity_weq; reflexivity.
+  + intros; apply <- wrap_identity_weq; reflexivity.
+  + intros; apply <- wrap_identity_weq; reflexivity.
 Defined.
 
 Definition identity_bind
@@ -68,14 +172,14 @@ Definition identity_bind
            (x:   Identity a)
            (f:   a -> Identity b)
   : Identity b :=
-  f x.
+  f (!x).
 
 Instance identity_Bind
   : Bind Identity :=
   { bind := identity_bind
   }.
 Proof.
-  + reflexivity.
+  + intros; apply wrap_identity_weq; reflexivity.
 Defined.
 
 Instance identity_Monad
@@ -83,6 +187,6 @@ Instance identity_Monad
   {
   }.
 Proof.
-  + reflexivity.
-  + reflexivity.
+  + intros; apply wrap_identity_weq; reflexivity.
+  + intros; apply <- wrap_identity_weq; reflexivity.
 Defined.
