theories/Control/State.v
@@ -11,16 +11,69 @@ Local Close Scope nat_scope.
 Local Open Scope free_control_scope.
 Local Open Scope free_weq_scope.
 
+(** * Definition
+
+ *)
+
 Definition StateT
            (s: Type)
            (m: Type -> Type)
-          `{Monad m}
+           `{Monad m}
            (a: Type)
-  := s -> m (a * s).
+  : Type :=
+  s -> m (a * s).
 
-Definition State
-           (s: Type) :=
-  StateT s Identity.
+Definition runStateT
+           {m: Type -> Type}
+          `{Monad m}
+           {s a: Type}
+           (ps:  StateT s m a)
+           (x:   s)
+  : m (a * s) :=
+  ps x.
+
+Definition evalStateT
+           {m: Type -> Type}
+          `{Monad m}
+           {s a: Type}
+           (ps:  StateT s m a)
+           (x:   s)
+  : m a :=
+  fst <$> runStateT ps x.
+
+Definition execStateT
+           {m: Type -> Type}
+          `{Monad m}
+           {s a: Type}
+           (ps:  StateT s m a)
+           (x:   s)
+  : m s :=
+  snd <$> runStateT ps x.
+
+(** * Monadic Interface
+
+ *)
+
+Definition get
+           {m: Type -> Type}
+          `{Monad m}
+           {s: Type}
+  : StateT s m s :=
+  fun x
+  => pure (x, x).
+
+Definition put
+           {m: Type -> Type}
+          `{Monad m}
+           {s: Type}
+           (x: s)
+  : StateT s m unit :=
+  fun _
+  => pure (tt, x).
+
+(** * State Monad
+
+ *)
 
 Definition state_map
            {m: Type -> Type}
@@ -30,25 +83,128 @@ Definition state_map
            (f:   a -> b)
            (fs:  StateT s m a)
   : StateT s m b :=
-  fun s
-  => o <- fs s                                                      ;
-     pure (f (fst o), (snd o)).
+    fun s
+    => o <- fs s                                                     ;
+       pure (f (fst o), (snd o)).
+
+Definition statet_weq
+           {m: Type -> Type}
+          `{Monad m}
+           {s:   Type}
+          `{WEq s}
+           {a: Type}
+          `{WEq a}
+           (p g: StateT s m a)
+  : Prop :=
+  forall (x: s),
+    fst <$> p x == fst <$> g x
+    /\ snd <$> p x == snd <$> g x.
+
+Lemma statet_weq_refl
+      {m: Type -> Type}
+     `{Monad m}
+      {s:   Type}
+     `{WEq s}
+      {a: Type}
+     `{WEq a}
+      (p: StateT s m a)
+  : statet_weq p p.
+Proof.
+  split.
+  + reflexivity.
+  + reflexivity.
+Qed.
+
+Lemma statet_weq_sym
+      {m: Type -> Type}
+     `{Monad m}
+      {s:   Type}
+     `{WEq s}
+      {a: Type}
+     `{WEq a}
+      (p q: StateT s m a)
+  : statet_weq p q
+    -> statet_weq q p.
+Proof.
+  intros G x.
+  assert (G': fst <$> p x == fst <$> q x /\ snd <$> p x == snd <$> q x)
+    by exact (G x).
+  destruct G' as [G1 G2].
+  split; symmetry; [ exact G1
+                   | exact G2
+                   ].
+Qed.
+
+Lemma statet_weq_trans
+      {m: Type -> Type}
+     `{Monad m}
+      {s:   Type}
+     `{WEq s}
+      {a: Type}
+     `{WEq a}
+      (p q r: StateT s m a)
+  : statet_weq p q
+    -> statet_weq q r
+    -> statet_weq p r.
+Proof.
+  intros Q R x.
+  assert (Q': fst <$> p x == fst <$> q x /\ snd <$> p x == snd <$> q x)
+    by exact (Q x).
+  assert (R': fst <$> q x == fst <$> r x /\ snd <$> q x == snd <$> r x)
+    by exact (R x).
+  destruct Q' as [Q1 Q2].
+  destruct R' as [R1 R2].
+  split.
+  + rewrite Q1; exact R1.
+  + rewrite Q2; exact R2.
+Qed.
+
+Add Parametric Relation
+    (m: Type -> Type)
+   `{Monad m}
+    (s:   Type)
+   `{WEq s}
+    (a: Type)
+   `{WEq a}
+  : (StateT s m a) (statet_weq)
+    reflexivity proved by statet_weq_refl
+    symmetry proved by statet_weq_sym
+    transitivity proved by statet_weq_trans
+      as statet_weq_equiv.
+
+Instance statet_WEq
+         (m: Type -> Type)
+        `{Monad m}
+         (s:   Type)
+        `{WEq s}
+         (a: Type)
+        `{WEq a}
+  : WEq (StateT s m a) :=
+  { weq := statet_weq
+  }.
 
 Lemma state_functor_identity
       (m: Type -> Type)
      `{Monad m}
       {s: Type}
+     `{WEq s}
       {a: Type}
+     `{WEq a}
       (ps: StateT s m a)
   : state_map _ _ id ps == id ps.
 Proof.
+  constructor.
+  + unfold state_map.
+    unfold id.
 Admitted.
 
 Lemma state_functor_composition_identity
       (m: Type -> Type)
      `{Monad m}
       {s: Type}
+     `{WEq s}
       {a b c: Type}
+     `{WEq c}
       (u: a -> b)
       (v: b -> c)
       (ps: StateT s m a)
@@ -60,6 +216,7 @@ Instance state_Functor
          (m: Type -> Type)
         `{Monad m}
          (s: Type)
+        `{WEq s}
   : Functor (StateT s m) :=
   { map := state_map
   }.
@@ -85,7 +242,9 @@ Lemma state_apply_composition
       (m: Type -> Type)
      `{Monad m}
       {s: Type}
+     `{WEq s}
       (a b c : Type)
+     `{WEq c}
       (u: StateT s m (b -> c))
       (v: StateT s m (a -> b))
       (w : StateT s m a):
@@ -98,6 +257,7 @@ Instance state_Apply
          (m: Type -> Type)
         `{Monad m}
          (s: Type)
+        `{WEq s}
   : Apply (StateT s m) :=
   { apply := state_apply
   }.
@@ -115,13 +275,15 @@ Definition state_bind
   : StateT s m b :=
   fun x
   => u <- fs x                                                       ;
-     pure (f (fst u)) (snd u).
+     f (fst u) (snd u).
 
 Lemma state_bind_associativity
       (m: Type -> Type)
      `{Monad m}
       {s: Type}
+     `{WEq s}
       (a b c : Type)
+     `{WEq c}
       (f : StateT s m a)
       (g : a -> StateT s m b)
       (h : b -> StateT s m c)
@@ -134,6 +296,7 @@ Instance state_Bind
          (m: Type -> Type)
         `{Monad m}
          (s: Type)
+        `{WEq s}
   : Bind (StateT s m) :=
   { bind := state_bind
   }.
@@ -151,20 +314,24 @@ Definition state_pure
   fun t => pure (x, t).
 
 Lemma state_applicative_identity
-      (m: Type -> Type)
+      {m: Type -> Type}
      `{Monad m}
       {s: Type}
+     `{WEq s}
       {a : Type}
+     `{WEq a}
       (v : StateT s m a):
   state_pure (a -> a) id <*> v == v.
 Proof.
 Admitted.
 
 Lemma state_applicative_composition
-      (m: Type -> Type)
+      {m: Type -> Type}
      `{Monad m}
       {s: Type}
+     `{WEq s}
       {a b c : Type}
+     `{WEq c}
       (u : StateT s m (b -> c))
       (v : StateT s m (a -> b))
       (w : StateT s m a)
@@ -174,13 +341,15 @@ Proof.
 Admitted.
 
 Lemma state_applicative_homomorphism
-      (m: Type -> Type)
+      {m: Type -> Type}
      `{Monad m}
       {s: Type}
+     `{WEq s}
       {a b: Type}
-      (v : a -> b)
-      (x : a)
-  : state_pure (s:=s) (a -> b) v <*> state_pure a x == state_pure b (v x).
+     `{WEq b}
+      (v: a -> b)
+      (x: a)
+  : state_pure _ v <*> state_pure _ x == (state_pure _ (v x): StateT s m b).
 Proof.
 Admitted.
 
@@ -188,7 +357,9 @@ Lemma state_applicative_interchange
       (m: Type -> Type)
      `{Monad m}
       {s: Type}
+     `{WEq s}
       (a b : Type)
+     `{WEq b}
       (u : StateT s m (a -> b))
       (y : a)
   : u <*> state_pure a y
@@ -200,21 +371,24 @@ Instance state_Applicative
          (m: Type -> Type)
         `{Monad m}
          (s: Type)
+        `{WEq s}
   : Applicative (StateT s m) :=
   { pure := state_pure
   }.
 Proof.
-  + apply state_applicative_identity.
-  + apply state_applicative_composition.
-  + apply state_applicative_homomorphism.
-  + apply state_applicative_interchange.
+  + apply (@state_applicative_identity m H s H0).
+  + apply (@state_applicative_composition m H s H0).
+  + apply (@state_applicative_homomorphism m H s H0).
+  + apply (@state_applicative_interchange m H s H0).
 Defined.
 
 Lemma state_monad_left_identity
       (m: Type -> Type)
      `{Monad m}
       {s: Type}
+     `{WEq s}
       (a b : Type)
+     `{WEq b}
       (x : a)
       (f : a -> StateT s m b)
   : (a <- pure x; f a) == f x.
@@ -225,7 +399,9 @@ Lemma state_monad_right_identity
       (m: Type -> Type)
      `{Monad m}
       {s: Type}
+     `{WEq s}
       (a : Type)
+     `{WEq a}
       (x : StateT s m a)
   : (y <- x; pure y) == x.
 Proof.
@@ -235,6 +411,7 @@ Instance state_Monad
          (m: Type -> Type)
         `{Monad m}
          (s: Type)
+        `{WEq s}
   : Monad (StateT s m) :=
   {
   }.
@@ -256,50 +433,15 @@ Definition state_lift
 
 Instance state_MonadTrans
          (s: Type)
+        `{WEq s}
   : MonadTrans (StateT s) :=
   { lift := state_lift s
   }.
 
-Definition runState
-           {m: Type -> Type}
-          `{Monad m}
-           {s a: Type}
-           (ps:  StateT s m a)
-           (x:   s)
-  : m (a * s) :=
-  ps x.
+(** * Pure Monad State
 
-Definition evalState
-           {m: Type -> Type}
-          `{Monad m}
-           {s a: Type}
-           (ps:  StateT s m a)
-           (x:   s)
-  : m a :=
-  fst <$> runState ps x.
+ *)
 
-Definition execState
-           {m: Type -> Type}
-          `{Monad m}
-           {s a: Type}
-           (ps:  StateT s m a)
-           (x:   s)
-  : m s :=
-  snd <$> runState ps x.
-
-Definition get
-           {m: Type -> Type}
-          `{Monad m}
-           {s: Type}
-  : StateT s m s :=
-  fun x
-  => pure (x, x).
-
-Definition put
-           {m: Type -> Type}
-          `{Monad m}
-           {s: Type}
-           (x: s)
-  : StateT s m unit :=
-  fun _
-  => pure (tt, x).
+Definition State
+           (s: Type) :=
+  StateT s Identity.
